Borrow Check: progress in defining function of computing the flow_kinds of generic origins in ADT

rustexamples/test/borrow_test/32.rs
@@ -14,23 +14,38 @@
 fn main(){
     let v1 : i32 = 22;
     let v2 : i32 = 44;
-    let p2: &mut i32 = &mut v2; // 'p2 -> {v2}
-    let p1: &mut i32 = &mut v1; // 'p1 -> {v1}, 'p2 -> {v2}
-    let q1: &mut &mut i32 = &mut p1; // 'q1 -> {p1}, ['p1, 'q2] -> {v1}, 'p2 -> {v2}
+    let p1: &mut i32 = &mut v1; // ['p1] -> {v1}
+    let p2: &mut i32 = &mut v2; // ['p1] -> {v1}, ['p2] -> {v2}
+    let q: &mut &mut i32 = &mut p1; // ['q1] -> {p1}, ['p1, 'q2] -> {v1}, ['p2] -> {v2}
     if true {
-        *p1 = 3; // 'q1 -> Invalid, ['p1, 'q2] -> {v1}, 'p2 -> {v2}
-        // p2 = &mut v2; // we cannot put p2 early because &mut v2 in the else branch would invalidate p2
-        q1 = &mut p2; // 'q1 -> {p2}, ['q2, 'p2] -> {v2}, 'p1 -> {v1}
+        // Steps of transfer in line :
+        // 1. apply liveness: remove 'q1 and 'q2 as q1 is dead, which produces ['p1] -> {v1}, ['p2] -> {v2}
+        // 2. access *p1 mutably: OK because *p1 is not an active loan
+        // 3. apply liveness: remove 'p1 as p1 is dead after this line, which produces ['p2] -> {v2} (TODO: we should talk about why we need this liveness application after the main transfer)
+        *p1 = 3; // ['p2] -> {v2}
+        q = &mut p2; // ['q1] -> {p2}, ['q2, 'p2] -> {v2}
     } else {
-        *q1 = &mut *p2; // 'q1 -> {p1}, ['p1, 'q2] -> {v1, v2, *p2}, 'p2 -> {v2}
-        // v1 = 13;
-        // *p1 = 5;
+        *q = &mut *p2; // ['q1] -> {p1}, ['p1, 'q2] -> {v1, v2, *p2}, ['p2] -> {v2}
     } // 'q1 -> {p1, p2}, ['p1, 'p2, 'q2] -> {v1, v2, *p2}
     v1 = 13; // 'q1 -> {p1, p2}, ['p1, 'p2, 'q2] -> Invalid
              // After this line, using places containing one of 'p1, 'p2 and 'q2 would cause error
-    // *p1 = 3;
+    *p1 = 3;
     *p2 = 3;
-     **q1 = 5;
-    *p2 = 5; // error
-    **q1 = 3; // error
+
+}
+
+
+fn test(){
+    let v1 : i32 = 22;
+    let v2 : i32 = 44;
+    let p1: &mut i32 = &mut v1; // ['p1] -> {v1}
+    let p2: &mut i32 = &mut v2; // ['p1] -> {v1}, ['p2] -> {v2}
+    let q: &mut &mut i32 = &mut p1; // ['q1] -> {p1}, ['p1, 'q2] -> {v1}, ['p2] ->  {v2}
+    if true {
+        q = &mut p2;
+    }
+    else {
+        *q = &mut v2;
+        p2 = &mut v1;
+    }
 }
